Ugly proof of the hard cases of LLL

raft/proof/LogsLeaderLogsProof.v
@@ -8,19 +8,898 @@ Require Import Net.
 Require Import Raft.
 Require Import RaftRefinementInterface.
 Require Import CommonDefinitions.
+Require Import CommonTheorems.
+
+Require Import SpecLemmas.
+
+Require Import UpdateLemmas.
+Local Arguments update {_} {_} {_} _ _ _ _ : simpl never.
+
 
 Require Import LogsLeaderLogsInterface.
+Require Import LeaderLogsSortedInterface.
+Require Import LeaderLogsContiguousInterface.
+Require Import LeaderLogsLogMatchingInterface.
+Require Import RefinedLogMatchingLemmasInterface.
+Require Import NextIndexSafetyInterface.
+Require Import SortedInterface.
 
 Section LogsLeaderLogs.
   Context {orig_base_params : BaseParams}.
   Context {one_node_params : OneNodeParams orig_base_params}.
   Context {raft_params : RaftParams orig_base_params}.
 
+  Context {rri : raft_refinement_interface}.
+  Context {llsi : leaderLogs_sorted_interface}.
+  Context {rlmli : refined_log_matching_lemmas_interface}.
+  Context {llci : leaderLogs_contiguous_interface}.
+  Context {lllmi : leaderLogs_entries_match_interface}.
+  Context {nisi : nextIndex_safety_interface}.
+  Context {si : sorted_interface}.
+
+  Definition logs_leaderLogs_nw net :=
+    forall p t n pli plt es ci e,
+      In p (nwPackets net) ->
+      pBody p = AppendEntries t n pli plt es ci ->
+      In e es ->
+      exists leader ll es' ll',
+        In (eTerm e, ll) (leaderLogs (fst (nwState net leader))) /\
+        Prefix ll' ll /\
+        removeAfterIndex es (eIndex e) = es' ++ ll' /\
+        (forall e', In e' es' -> eTerm e' = eTerm e) /\
+        ((plt = eTerm e /\ pli > maxIndex ll)  \/
+         (exists e, In e ll /\ eIndex e = pli /\ eTerm e = plt /\ (ll' <> [] \/
+                                                             pli = maxIndex ll)) \/
+         plt = 0 /\ pli = 0).
+
+
+  Definition logs_leaderLogs_nw_weak net :=
+    forall p t n pli plt es ci e,
+      In p (nwPackets net) ->
+      pBody p = AppendEntries t n pli plt es ci ->
+      In e es ->
+      exists leader ll es' ll',
+        In (eTerm e, ll) (leaderLogs (fst (nwState net leader))) /\
+        Prefix ll' ll /\
+        removeAfterIndex es (eIndex e) = es' ++ ll' /\
+        (forall e', In e' es' -> eTerm e' = eTerm e).
+
+  Lemma logs_leaderLogs_nw_weaken :
+    forall net,
+      logs_leaderLogs_nw net ->
+      logs_leaderLogs_nw_weak net.
+  Proof.
+    intros. unfold logs_leaderLogs_nw, logs_leaderLogs_nw_weak in *.
+    intros.
+    eapply_prop_hyp In In; eauto.
+    break_exists_exists; intuition.
+  Qed.
+    
+  Definition logs_leaderLogs_inductive net :=
+    logs_leaderLogs net /\
+    logs_leaderLogs_nw net.
+
+  Theorem lift_sorted :
+    forall net,
+      refined_raft_intermediate_reachable net ->
+      logs_sorted (deghost net).
+  Proof.
+    intros.
+    eapply lift_prop; eauto using logs_sorted_invariant.
+  Qed.
+  
+  Theorem lift_logs_sorted :
+    forall net h,
+      refined_raft_intermediate_reachable net ->
+      sorted (log (snd (nwState net h))).
+  Proof.
+    intros.
+    find_apply_lem_hyp lift_sorted.
+    unfold logs_sorted, logs_sorted_host in *.
+    intuition.
+    unfold deghost in *. simpl in *. break_match; eauto.
+  Qed.
+
+  Lemma lift_nextIndex_safety :
+    forall net,
+      refined_raft_intermediate_reachable net ->
+      nextIndex_safety (deghost net).
+  Proof.
+    intros.
+    eapply lift_prop; eauto using nextIndex_safety_invariant.
+  Qed.
+
+  Require Import Omega.
+  
+  Lemma nextIndex_sanity :
+    forall net h h',
+      refined_raft_intermediate_reachable net ->
+      type (snd (nwState net h)) = Leader ->
+      pred (getNextIndex (snd (nwState net h)) h') <> 0 ->
+      exists e,
+        findAtIndex (log (snd (nwState net h))) (pred (getNextIndex (snd (nwState net h)) h')) = Some e.
+  Proof.
+    intros.
+    find_copy_apply_lem_hyp entries_contiguous_invariant.
+    find_copy_apply_lem_hyp lift_nextIndex_safety.
+    assert (pred (getNextIndex (snd (nwState net h)) h') > 0) by omega.
+    unfold nextIndex_safety in *.
+    match goal with
+      | H : forall _ _, type _ = _ -> _ |- _ => specialize (H h h')
+    end. 
+    intuition.
+    unfold entries_contiguous in *. specialize (H2 h).
+    unfold contiguous_range_exact_lo in *. intuition.
+    match goal with
+      | H : forall _, _ < _ <= _ -> _ |- _ =>
+        specialize (H (pred (getNextIndex (snd (nwState net h)) h')))
+    end.
+    unfold raft_refined_base_params in *.
+    repeat find_rewrite_lem deghost_spec. intuition.
+    break_exists_exists. intuition.
+    apply findAtIndex_intro; eauto using lift_logs_sorted, sorted_uniqueIndices.
+  Qed.
+
+  
+  Lemma update_elections_data_client_request_leaderLogs :
+    forall h st client id c,
+      leaderLogs (update_elections_data_client_request h st client id c) =
+      leaderLogs (fst st).
+  Proof.
+    unfold update_elections_data_client_request in *.
+    intros. repeat break_match; repeat find_inversion; auto.
+  Qed.
+
+  Lemma update_elections_data_timeout_leaderLogs :
+    forall h st,
+      leaderLogs (update_elections_data_timeout h st) =
+      leaderLogs (fst st).
+  Proof.
+    unfold update_elections_data_timeout.
+    intros.
+    repeat break_match; simpl in *; auto.
+  Qed.
+
+  Lemma update_elections_data_appendEntries_leaderLogs :
+    forall h st t h' pli plt es ci,
+      leaderLogs (update_elections_data_appendEntries h st t h' pli plt es ci) =
+      leaderLogs (fst st).
+  Proof.
+    intros.
+    unfold update_elections_data_appendEntries.
+    repeat break_match; subst; simpl in *; auto.
+  Qed.
+  
+  Lemma update_elections_data_requestVote_leaderLogs :
+    forall h h' t lli llt st,
+      leaderLogs (update_elections_data_requestVote h h' t h' lli llt st) =
+      leaderLogs (fst st).
+  Proof.
+    unfold update_elections_data_requestVote.
+    intros.
+    repeat break_match; auto.
+  Qed.
+
+  Lemma update_elections_data_requestVoteReply_leaderLogs :
+    forall h h' t  st t' ll' r,
+      In (t', ll') (leaderLogs (fst st)) ->
+      In (t', ll') (leaderLogs (update_elections_data_requestVoteReply h h' t r st)).
+  Proof.
+    unfold update_elections_data_requestVoteReply.
+    intros.
+    repeat break_match; auto.
+    simpl in *. intuition.
+  Qed.
+  
+
+  Ltac prove_in :=
+    match goal with
+      | [ _ : nwPackets ?net = _,
+              _ : In (?p : packet) _ |- _] =>
+        assert (In p (nwPackets net)) by (repeat find_rewrite; do_in_app; intuition)
+      | [ _ : nwPackets ?net = _,
+              _ : pBody ?p = _ |- _] =>
+        assert (In p (nwPackets net)) by (repeat find_rewrite; intuition)
+    end.
+
+  Ltac update_destruct :=
+    match goal with
+    | [ |- context [ update _ ?y _ ?x ] ] => destruct (name_eq_dec y x)
+    end.
+  
+  Require Import Omega.
+
+  Lemma sorted_Prefix_in_eq :
+    forall l' l,
+      sorted l ->
+      Prefix l' l ->
+      (forall e, In e l -> In e l') ->
+      l' = l.
+  Proof.
+    induction l'; intros; simpl in *; intuition.
+    - destruct l; simpl in *; auto.
+      specialize (H1 e); intuition.
+    - break_match; intuition. subst.
+      simpl in *. intuition. f_equal.
+      eapply IHl'; eauto.
+      intros.
+      specialize (H1 e0); intuition.
+      subst. specialize (H0 e0); intuition. omega.
+  Qed.
+
+  Lemma removeAfterIndex_eq :
+    forall l i,
+      (forall e, In e l -> eIndex e <= i) ->
+      removeAfterIndex l i = l.
+  Proof.
+    induction l; intros; simpl in *; intuition.
+    break_if; intuition.
+    do_bool. specialize (H a). intuition. omega.
+  Qed.
+
+  Lemma thing2 :
+    forall l l' i,
+      l <> [] ->
+      Prefix l l' ->
+      sorted l' ->
+      contiguous_range_exact_lo l i ->
+      contiguous_range_exact_lo l' 0 ->
+      l ++ (removeAfterIndex l' i) = l'.
+  Proof.
+    admit.
+  Qed.
+
+  Lemma thing :
+    forall es l l' e e',
+      sorted l ->
+      sorted l' ->
+      entries_match l l' ->
+      es <> [] ->
+      Prefix es l' ->
+      contiguous_range_exact_lo es (eIndex e) ->
+      In e l ->
+      In e' l' ->
+      eIndex e = eIndex e' ->
+      eTerm e = eTerm e' ->
+      es ++ (removeAfterIndex l (eIndex e)) = l'.
+  Proof.
+  Admitted.
+    
+  Lemma removeAfterIndex_in_app :
+    forall l l' e,
+      In e l ->
+      removeAfterIndex (l ++ l') (eIndex e) =
+      (removeAfterIndex l (eIndex e)) ++ l'.
+  Proof.
+    induction l; intros; simpl in *; intuition;
+    subst; break_if; do_bool; eauto using app_ass.
+    omega.
+  Qed.
+
+  Lemma removeAfterIndex_in_app_l' :
+    forall l l' e,
+      (forall e', In e' l -> eIndex e' > eIndex e) ->
+      In e l' ->
+      removeAfterIndex (l ++ l') (eIndex e) =
+      removeAfterIndex l' (eIndex e).
+  Proof.
+    induction l; intros; simpl in *; intuition;
+    subst; break_if; do_bool; eauto using app_ass.
+    specialize (H a). intuition. omega.
+  Qed.
+
+  Lemma removeAfterIndex_maxIndex_sorted :
+    forall l,
+      sorted l ->
+      l = removeAfterIndex l (maxIndex l).
+  Proof.
+    intros; induction l; simpl in *; intuition.
+    break_if; auto. do_bool. omega.
+  Qed.
+
+  Lemma logs_leaderLogs_inductive_appendEntries :
+    refined_raft_net_invariant_append_entries logs_leaderLogs_inductive.
+  Proof.
+    red. unfold logs_leaderLogs_inductive. intros.
+    subst. simpl in *. intuition.
+    - unfold logs_leaderLogs in *. intros.
+      simpl in *. repeat find_higher_order_rewrite.
+      update_destruct; subst; rewrite_update; eauto.
+      + simpl in *. find_apply_lem_hyp handleAppendEntries_log.
+        intuition; repeat find_rewrite; eauto.
+        * find_apply_hyp_hyp. break_exists_exists; intuition.
+          find_higher_order_rewrite; update_destruct; subst; rewrite_update; eauto.
+          simpl in *.
+          rewrite update_elections_data_appendEntries_leaderLogs. auto.
+        * { subst.
+            find_apply_lem_hyp logs_leaderLogs_nw_weaken.
+            unfold logs_leaderLogs_nw_weak in *.
+            copy_eapply_prop_hyp pBody pBody; eauto.
+            break_exists_exists.
+            break_exists. intuition.
+            - repeat find_higher_order_rewrite.
+              update_destruct; subst; rewrite_update; eauto.
+              simpl.
+              rewrite update_elections_data_appendEntries_leaderLogs.
+              auto.
+            - repeat find_rewrite. f_equal.
+              find_copy_apply_lem_hyp leaderLogs_sorted_invariant; eauto.
+              eapply sorted_Prefix_in_eq; eauto.
+              intros.
+              eapply prefix_contiguous with (i := 0); eauto.
+              + eapply leaderLogs_contiguous_invariant; eauto.
+              + assert (sorted (log d)) by (eapply entries_sorted_nw_invariant; eauto).
+                eapply contiguous_app with (l1 := x1).
+                * repeat find_reverse_rewrite.
+                  apply removeAfterIndex_sorted. auto.
+                * repeat find_reverse_rewrite.
+                  eapply removeAfterIndex_contiguous; eauto.
+                  eapply entries_contiguous_nw_invariant; eauto.
+          }
+        * { break_exists. intuition. subst.
+            do_in_app. intuition.
+            - (* new entry *)
+              unfold logs_leaderLogs_nw in *.
+              prove_in.
+              copy_eapply_prop_hyp In In; eauto.
+              match goal with
+                | H:exists _, _ |- _ => destruct H as (leader)
+              end.
+              break_exists; intuition.
+              + (* all of the new entries, as well as x, are in the
+                new term. This means we can apply the host invariant
+                to x and get our leader. *)
+                assert (x2 = []).
+                {
+                  destruct x2; intuition. exfalso.
+                  simpl in *. break_match; intuition.
+                  simpl in *. subst.
+                  find_copy_apply_lem_hyp entries_contiguous_nw_invariant.
+                  eapply_prop_hyp entries_contiguous_nw pBody; eauto.
+                  unfold contiguous_range_exact_lo in *. intuition.
+                  match goal with
+                    | _ : removeAfterIndex _ ?index = _ ++ ?e :: _ |- _ =>
+                      assert (In e es) by
+                          (apply removeAfterIndex_in with (i := index);
+                           repeat find_rewrite; intuition)
+                  end.
+                  eapply_prop_hyp In In. omega.
+                } subst. rewrite app_nil_r in *.
+                match goal with
+                  | H : forall _ _, In _ _ -> _ |- _ =>
+                    specialize (H0 (pDst p) x)
+                end. intuition.
+                break_exists. intuition.
+                match goal with
+                  | _ : In (_, ?ll) (leaderLogs (_ (_ _ ?h))),
+                        _ : removeAfterIndex _ _ = ?es' ++ ?ll |- _ =>
+                    exists h, ll, (removeAfterIndex es (eIndex e) ++ es')
+                end. intuition.
+                * repeat find_rewrite.
+                  match goal with
+                    | H : forall _, st' _ = _ |- _ =>
+                      rewrite H
+                  end.
+                  update_destruct; subst; rewrite_update; eauto.
+                  simpl in *.
+                  rewrite update_elections_data_appendEntries_leaderLogs. auto.
+                * rewrite removeAfterIndex_in_app; auto.
+                  rewrite app_ass. repeat find_rewrite. auto.
+                * repeat find_rewrite. do_in_app. intuition; eauto.
+              + (* we share an entry with the leader, so we can use
+                log matching to make sure our old entries match. we'll
+                get the new entries for free from the nw invariant. *)
+                break_exists; intuition;
+                match goal with
+                  | [ _ : In (_, ?ll) (leaderLogs (_ (_ _ ?leader))),
+                      _ : removeAfterIndex _ _ = ?es' ++ _ |- _ ] =>
+                    exists leader, ll, es'
+                end; intuition.
+                * repeat find_rewrite.
+                  match goal with
+                    | H : forall _, st' _ = _ |- _ =>
+                      rewrite H
+                  end.
+                  update_destruct; subst; rewrite_update; eauto.
+                  simpl in *.
+                  rewrite update_elections_data_appendEntries_leaderLogs. auto.
+                * rewrite removeAfterIndex_in_app; auto.
+                  repeat find_rewrite. rewrite app_ass.
+                  find_copy_eapply_lem_hyp leaderLogs_sorted_invariant; eauto.
+                  f_equal.
+                  eapply thing; eauto using lift_logs_sorted;
+                  [eapply leaderLogs_entries_match_invariant; eauto|].
+                  assert (sorted es) by (eapply entries_sorted_nw_invariant; eauto).
+                  find_copy_apply_lem_hyp entries_contiguous_nw_invariant.
+                  unfold entries_contiguous_nw in *.
+                  copy_eapply_prop_hyp contiguous_range_exact_lo pBody; eauto.
+                  find_eapply_lem_hyp removeAfterIndex_contiguous; eauto.
+                  match goal with
+                    | H : removeAfterIndex _ _ = _ |- _ =>
+                      find_erewrite_lem H
+                  end.
+                  eapply contiguous_app; eauto.
+                  repeat find_reverse_rewrite. eauto using removeAfterIndex_sorted.
+                * repeat find_rewrite.
+                  match goal with
+                    | H : forall _, st' _ = _ |- _ =>
+                      rewrite H
+                  end.
+                  update_destruct; subst; rewrite_update; eauto.
+                  simpl in *.
+                  rewrite update_elections_data_appendEntries_leaderLogs. auto.
+                * rewrite removeAfterIndex_in_app; auto.
+                  repeat find_rewrite. rewrite app_ass.
+                  f_equal.
+                  assert (x2 = []).
+                  {
+                    destruct x2; intuition. exfalso.
+                    simpl in *. break_match; intuition.
+                    simpl in *. subst.
+                    find_copy_apply_lem_hyp entries_contiguous_nw_invariant.
+                    eapply_prop_hyp entries_contiguous_nw pBody; eauto.
+                    unfold contiguous_range_exact_lo in *. break_and.
+                    match goal with
+                      | _ : removeAfterIndex _ ?index = _ ++ ?e :: _ |- _ =>
+                        assert (In e es) by
+                            (apply removeAfterIndex_in with (i := index);
+                             repeat find_rewrite; intuition)
+                    end.
+                    eapply_prop_hyp In In. omega.
+                  } subst. simpl.
+                  find_copy_eapply_lem_hyp leaderLogs_sorted_invariant; eauto.
+                  match goal with
+                    | |- _ = ?ll =>
+                      rewrite removeAfterIndex_maxIndex_sorted with (l := ll) at 2
+                  end; eauto.
+                  eapply removeAfterIndex_same_sufficient; eauto using lift_logs_sorted;
+                  intros;
+                  match goal with
+                    | _ : eIndex ?e = maxIndex _,
+                          _ : In ?e (log _),
+                              _ : eIndex ?e' = maxIndex _ |- In ?e'' _ =>
+                      assert (eIndex e = eIndex e') as Heq by (repeat find_rewrite; auto);
+                        assert (eIndex e'' <= eIndex e) by omega;
+                        eapply leaderLogs_entries_match_invariant in Heq; eauto;
+                        repeat conclude Heq ltac:(eauto; intuition)
+                  end; intuition.
+            - (* old entry *)
+              (* can use host invariant, since we don't change removeAfterIndex *)
+              find_copy_apply_lem_hyp removeAfterIndex_in.
+              find_copy_apply_lem_hyp removeAfterIndex_In_le; eauto using lift_logs_sorted.
+              find_apply_hyp_hyp. break_exists_exists; intuition.
+              + find_higher_order_rewrite; update_destruct; subst; rewrite_update; eauto.
+                simpl in *.
+                rewrite update_elections_data_appendEntries_leaderLogs. auto.
+              + rewrite removeAfterIndex_in_app_l'; eauto;
+                [rewrite <- removeAfterIndex_le; auto|].
+                intros. eapply gt_le_trans; [|eauto].
+                eapply entries_contiguous_nw_invariant; eauto.
+          }
+      + find_apply_hyp_hyp. break_exists_exists; intuition.
+        find_higher_order_rewrite; update_destruct; subst; rewrite_update; eauto.
+        simpl in *.
+        rewrite update_elections_data_appendEntries_leaderLogs. auto.
+    - unfold logs_leaderLogs_nw in *.
+      intros. simpl in *. find_apply_hyp_hyp.
+      intuition.
+      + prove_in.
+        copy_eapply_prop_hyp In In; eauto.
+        break_exists_exists; intuition;
+        repeat find_higher_order_rewrite;
+        update_destruct; subst; rewrite_update; eauto;
+        simpl in *;
+        rewrite update_elections_data_appendEntries_leaderLogs; auto.
+      + exfalso. subst. simpl in *.
+        unfold handleAppendEntries in *; repeat break_match; find_inversion; congruence.
+  Qed.
+  
+  Lemma logs_leaderLogs_inductive_appendEntriesReply :
+    refined_raft_net_invariant_append_entries_reply logs_leaderLogs_inductive.
+  Proof.
+    admit.
+  Qed.
+
+
+  Lemma logs_leaderLogs_inductive_requestVote :
+    refined_raft_net_invariant_request_vote logs_leaderLogs_inductive.
+  Proof.
+    admit.
+  Qed.
+  
+  Lemma logs_leaderLogs_inductive_requestVoteReply :
+    refined_raft_net_invariant_request_vote_reply logs_leaderLogs_inductive.
+  Proof.
+    admit.
+  Qed.
+
+  Lemma logs_leaderLogs_inductive_clientRequest :
+    refined_raft_net_invariant_client_request logs_leaderLogs_inductive.
+  Proof.
+    admit.
+  Qed.
+  
+  Lemma logs_leaderLogs_inductive_timeout :
+    refined_raft_net_invariant_timeout logs_leaderLogs_inductive.
+  Proof.
+    admit.
+  Qed.
+
+  Lemma logs_leaderLogs_inductive_doGenericServer :
+    refined_raft_net_invariant_do_generic_server logs_leaderLogs_inductive.
+  Proof.
+    admit.
+  Qed.
+
+  Require Import PeanoNat.
+  Require Import Nat.
+
+  Lemma doLeader_spec :
+    forall st h os st' ms m t n pli plt es ci,
+      doLeader st h = (os, st', ms) ->
+      In m ms ->
+      snd m = AppendEntries t n pli plt es ci ->
+      t = currentTerm st /\
+      log st' = log st /\
+      type st = Leader /\
+      ((pli = 0 /\ plt = 0 /\ es = findGtIndex (log st) 0) \/
+       ((exists e, findAtIndex (log st) pli = Some e /\
+              eTerm e = plt) /\
+        es = findGtIndex (log st) pli) \/
+       exists h', pred (getNextIndex st h') <> 0 /\ findAtIndex (log st) (pred (getNextIndex st h')) = None).
+  Proof.
+    intros. unfold doLeader, advanceCommitIndex in *.
+    break_match; try solve [find_inversion; simpl in *; intuition].
+    break_if; try solve [find_inversion; simpl in *; intuition].
+    find_inversion. simpl. do_in_map. subst.
+    simpl in *. find_inversion. intuition.
+    match goal with
+      | |- context [pred ?x] =>
+        remember (pred x) as index
+    end. break_match; simpl in *.
+    - right. left. eauto.
+    -  destruct index; intuition.
+       right. right. exists x.
+       match goal with
+         | _ : S _ = pred ?x |- context [pred ?y] =>
+           assert (pred x = pred y) by auto
+       end.
+       repeat find_rewrite. intuition.
+  Qed.
+
+  Lemma sorted_findGtIndex_0 :
+    forall l,
+      (forall e, In e l -> eIndex e > 0) ->
+      sorted l ->
+      findGtIndex l 0 = l.
+  Proof.
+    induction l; intros; simpl in *; intuition.
+    break_if; intuition.
+    - f_equal. auto.
+    - do_bool. specialize (H a); intuition; omega.
+  Qed.
+  
+  Lemma Prefix_refl :
+    forall A (l : list A),
+      Prefix l l.
+  Proof.
+    intros. induction l; simpl in *; auto.
+  Qed.
+
+  Require Import Omega.
+  
+  Lemma findGtIndex_app_in_1 :
+    forall l1 l2 e,
+      sorted (l1 ++ l2) ->
+      In e l1 ->
+      exists l',
+        findGtIndex (l1 ++ l2) (eIndex e) = l' /\
+        forall x,
+          In x l' -> In x l1.
+  Proof.
+    induction l1; intros; simpl in *; intuition.
+    - subst. break_if; do_bool; try omega.
+      eexists; repeat (simpl in *; intuition).
+    - specialize (H1 e); intuition. conclude H1 ltac:(apply in_app_iff; intuition).
+      break_if; do_bool; try omega. eexists; intuition; eauto.
+      simpl in *. intuition.
+      eapply_prop_hyp sorted sorted; eauto. break_exists; intuition.
+      find_rewrite. eauto.
+  Qed.
+  
+  Lemma sorted_app_in_1 :
+    forall l1 l2 e,
+      sorted (l1 ++ l2) ->
+      eIndex e > 0 ->
+      In e l1 ->
+      eIndex e > maxIndex l2.
+  Proof.
+    induction l1; intros; simpl in *; intuition.
+    subst. destruct l2; simpl in *; auto.
+    specialize (H2 e0); concludes; intuition.
+  Qed.
+
+  Lemma findGtIndex_Prefix :
+    forall l i,
+      Prefix (findGtIndex l i) l.
+  Proof.
+    induction l; intros; simpl in *; intuition.
+    break_if; simpl in *; intuition.
+  Qed.
+  
+  Lemma findGtIndex_app_in_2 :
+    forall l1 l2 e,
+      sorted (l1 ++ l2) ->
+      In e l2 ->
+      exists l',
+        findGtIndex (l1 ++ l2) (eIndex e) = l1 ++ l' /\
+        Prefix l' l2.
+  Proof.
+    induction l1; intros; simpl in *; intuition.
+    - eexists; intuition eauto using findGtIndex_Prefix.
+    - break_if; simpl in *; intuition.
+      + eapply_prop_hyp sorted sorted; eauto.
+        break_exists; intuition; find_rewrite; eauto.
+      + do_bool. specialize (H1 e); conclude H1 ltac:(apply in_app_iff; intuition).
+        omega.
+  Qed.
+  
+  Lemma logs_leaderLogs_inductive_doLeader :
+    refined_raft_net_invariant_do_leader logs_leaderLogs_inductive.
+  Proof.
+    red. unfold logs_leaderLogs_inductive. intros.
+    match goal with
+      | H : nwState ?net ?h = (?gd, ?d) |- _ =>
+        replace gd with (fst (nwState net h)) in * by (rewrite H; reflexivity);
+          replace d with (snd (nwState net h)) in * by (rewrite H; reflexivity);
+          clear H
+    end.
+    intuition.
+    - admit.
+    - unfold logs_leaderLogs_nw.
+      intros. simpl in *. find_apply_hyp_hyp.
+      break_or_hyp.
+      + admit.
+      + { do_in_map. subst. simpl in *.
+          find_eapply_lem_hyp doLeader_spec; eauto. intuition.
+          - subst. (* just use host invariant *)
+            unfold logs_leaderLogs in *.
+            find_apply_lem_hyp findGtIndex_necessary.
+            intuition.
+            eapply_prop_hyp In In.
+            break_exists_exists. intuition.
+            match goal with
+              | _ : In (_, ?ll) _ |- _ =>
+                exists ll
+            end.
+            intuition; eauto using Prefix_refl;
+            [find_higher_order_rewrite; update_destruct; subst; rewrite_update; eauto|].
+            rewrite sorted_findGtIndex_0; eauto using lift_logs_sorted.
+            intros. eapply entries_gt_0_invariant; eauto.
+          - break_exists. break_and.
+            subst.
+            unfold logs_leaderLogs in *.
+            find_apply_lem_hyp findGtIndex_necessary.
+            break_and. find_apply_hyp_hyp.
+            match goal with
+              | H : exists _ _ _, _ |- _ =>
+                destruct H as (leader);
+                  destruct H as (ll);
+                  destruct H as (es)
+            end.
+            break_and.
+            destruct (lt_eq_lt_dec (maxIndex ll) pli); intuition.
+            + exists leader, ll, (findGtIndex es pli), []. intuition.
+              * find_higher_order_rewrite; update_destruct; subst; rewrite_update; eauto.
+              * simpl; auto.
+              * rewrite app_nil_r.
+                Lemma findGtIndex_nil :
+                  forall l i,
+                    (forall e', In e' l -> eIndex e' <= i) ->
+                    findGtIndex l i = [].
+                Proof.
+                  intros; induction l; simpl in *; intuition.
+                  break_if; do_bool; intuition.
+                  specialize (H a); intuition. omega.
+                Qed.
+                Lemma findGtIndex_removeAfterIndex_commute :
+                  forall l i i',
+                    sorted l ->
+                    removeAfterIndex (findGtIndex l i) i' =
+                    findGtIndex (removeAfterIndex l i') i.
+                Proof.
+                  intros. induction l; simpl in *; auto.
+                  repeat (break_if; simpl; intuition); do_bool;
+                  try congruence.
+                  symmetry. apply findGtIndex_nil.
+                  intros. find_apply_lem_hyp removeAfterIndex_in.
+                  find_apply_hyp_hyp. intuition.
+                Qed.
+                rewrite findGtIndex_removeAfterIndex_commute; eauto using lift_logs_sorted.
+                unfold ghost_data in *. simpl in *.
+                find_rewrite.
+
+                Lemma findGtIndex_app_1 :
+                  forall l l' i,
+                    maxIndex l' <= i ->
+                    findGtIndex (l ++ l') i = findGtIndex l i.
+                Proof.
+                  induction l; intros; simpl in *; intuition.
+                  - destruct l'; simpl in *; intuition.
+                    break_if; do_bool; auto; omega.
+                  - break_if; do_bool; auto.
+                    f_equal. eauto.
+                Qed.
+                eapply findGtIndex_app_1; omega.
+              * eauto using findGtIndex_in.
+              * left. intuition.
+                match goal with
+                  | H : forall _, In _ _ -> _ |- _ =>
+                    apply H
+                end.
+                find_apply_lem_hyp findAtIndex_elim. intuition.
+                subst.
+                match goal with
+                  | _ : In ?x ?l, _ : eIndex ?e > eIndex ?x |- _ =>
+                    assert (In x (removeAfterIndex l (eIndex e))) by
+                        (apply removeAfterIndex_le_In; eauto; omega)
+                end.
+                unfold ghost_data in *. simpl in *.
+                find_rewrite.
+                do_in_app; intuition.
+                find_copy_apply_lem_hyp leaderLogs_sorted_invariant; eauto.
+                find_apply_lem_hyp maxIndex_is_max; eauto; omega.
+            + exists leader, ll, (findGtIndex es pli), []. intuition.
+              * find_higher_order_rewrite; update_destruct; subst; rewrite_update; eauto.
+              * simpl; auto.
+              * rewrite app_nil_r.
+                rewrite findGtIndex_removeAfterIndex_commute; eauto using lift_logs_sorted.
+                unfold ghost_data in *. simpl in *.
+                find_rewrite.
+                apply findGtIndex_app_1. omega.
+              * eauto using findGtIndex_in.
+              * right. find_apply_lem_hyp findAtIndex_elim.
+                left. exists x0. intuition. subst.
+                match goal with
+                  | _ : In ?x ?l, _ : eIndex ?e > _ |- _ =>
+                    assert (In x (removeAfterIndex l (eIndex e))) by
+                        (apply removeAfterIndex_le_In; eauto; omega)
+                end.
+                unfold ghost_data in *. simpl in *.
+                find_rewrite.
+                assert (sorted (es ++ ll)) by (repeat find_reverse_rewrite;
+                                               apply removeAfterIndex_sorted;
+                                               repeat find_rewrite; eauto using lift_logs_sorted).
+                Lemma thing3 :
+                  forall l l' e,
+                    sorted (l ++ l') ->
+                    (forall e', In e' (l ++ l') -> eIndex e' > 0) ->
+                    In e (l ++ l') ->
+                    eIndex e <= maxIndex l' ->
+                    In e l'.
+                Proof.
+                  induction l; intros; simpl in *; intuition.
+                  subst. destruct l'; simpl in *; intuition.
+                  - exfalso. specialize (H0 e). intuition.
+                  - exfalso. specialize (H3 e0). conclude_using intuition.
+                    intuition.
+                Qed.
+                eapply thing3; eauto; try omega. intros.
+                match goal with
+                  | |- eIndex ?e > _ =>
+                    assert (In e (log (snd (nwState net h)))) by
+                        (unfold ghost_data in *; simpl in *;
+                         eapply removeAfterIndex_in; repeat find_reverse_rewrite; eauto)
+                end. 
+                eapply entries_gt_0_invariant; eauto.
+            + exists leader, ll, es, (findGtIndex ll pli). intuition.
+              * find_higher_order_rewrite; update_destruct; subst; rewrite_update; eauto.
+              * (* prefix_findGtIndex *)
+                apply findGtIndex_Prefix.
+              * rewrite findGtIndex_removeAfterIndex_commute; eauto using lift_logs_sorted.
+                unfold ghost_data in *. simpl in *.
+                find_rewrite.
+                Lemma findGtIndex_app_2 :
+                  forall l l' i,
+                    sorted (l ++ l') ->
+                    i < maxIndex l' ->
+                    findGtIndex (l ++ l') i = l ++ findGtIndex l' i.
+                Proof.
+                  induction l; intros; simpl in *; intuition.
+                  break_if; do_bool; auto.
+                  - f_equal. eauto.
+                  - exfalso.
+                    destruct l'; simpl in *; intuition.
+                    specialize (H1 e); conclude_using intuition; intuition.
+                Qed.
+                assert (sorted (es ++ ll)) by (repeat find_reverse_rewrite;
+                                               apply removeAfterIndex_sorted;
+                                               repeat find_rewrite; eauto using lift_logs_sorted).
+                apply findGtIndex_app_2; auto.
+              * { right. left.
+                  find_apply_lem_hyp findAtIndex_elim. 
+                  exists x0.  intuition.
+                  - subst.
+                    match goal with
+                      | H : removeAfterIndex _ _ = _ |- _ =>
+                        find_eapply_lem_hyp removeAfterIndex_le_In;
+                          [unfold ghost_data in *; simpl in *; find_rewrite_lem H|omega]
+                    end.
+                    assert (sorted (es ++ ll)) by (repeat find_reverse_rewrite;
+                                                   apply removeAfterIndex_sorted;
+                                                   repeat find_rewrite; eauto using lift_logs_sorted).
+                    eapply thing3; eauto; try omega. intros.
+                     match goal with
+                       | |- eIndex ?e > _ =>
+                         assert (In e (log (snd (nwState net h)))) by
+                             (unfold ghost_data in *; simpl in *;
+                              eapply removeAfterIndex_in; repeat find_reverse_rewrite; eauto)
+                     end. 
+                     eapply entries_gt_0_invariant; eauto.
+                  - left. intros.
+                    Lemma findGtIndex_non_empty :
+                      forall l i,
+                        i < maxIndex l ->
+                        findGtIndex l i <> [].
+                    Proof.
+                      intros. induction l; simpl in *; intuition.
+                      break_if; do_bool; simpl in *; intuition.
+                      congruence.
+                    Qed.
+                    eapply findGtIndex_non_empty; eauto.
+                }
+          - exfalso. (* use nextIndex_sanity *)
+            break_exists. intuition.
+            find_eapply_lem_hyp nextIndex_sanity; eauto. break_exists.
+            unfold ghost_data in *. simpl in *. congruence.
+        }
+  Qed.
+
+  Lemma logs_leaderLogs_inductive_init :
+    refined_raft_net_invariant_init logs_leaderLogs_inductive.
+  Proof.
+    admit.
+  Qed.
+
+  Lemma logs_leaderLogs_inductive_state_same_packets_subset :
+    refined_raft_net_invariant_state_same_packet_subset logs_leaderLogs_inductive.
+  Proof.
+    admit.
+  Qed.
+
+  Lemma logs_leaderLogs_inductive_reboot :
+    refined_raft_net_invariant_reboot logs_leaderLogs_inductive.
+  Proof.
+    admit.
+  Qed.
+
+  Theorem logs_leaderLogs_inductive_invariant :
+    forall net,
+      refined_raft_intermediate_reachable net ->
+      logs_leaderLogs_inductive net.
+  Proof.
+    intros.
+    apply refined_raft_net_invariant; auto.
+    - apply logs_leaderLogs_inductive_init.
+    - apply logs_leaderLogs_inductive_clientRequest.
+    - apply logs_leaderLogs_inductive_timeout.
+    - apply logs_leaderLogs_inductive_appendEntries.
+    - apply logs_leaderLogs_inductive_appendEntriesReply.
+    - apply logs_leaderLogs_inductive_requestVote.
+    - apply logs_leaderLogs_inductive_requestVoteReply.
+    - apply logs_leaderLogs_inductive_doLeader.
+    - apply logs_leaderLogs_inductive_doGenericServer.
+    - apply logs_leaderLogs_inductive_state_same_packets_subset.
+    - apply logs_leaderLogs_inductive_reboot.
+  Qed.
+  
   Theorem logs_leaderLogs_invariant :
     forall net,
       refined_raft_intermediate_reachable net ->
       logs_leaderLogs net.
-  Admitted.
+  Proof.
+    intros. apply logs_leaderLogs_inductive_invariant. auto.
+  Qed.
 
   Instance llli : logs_leaderLogs_interface.
   Proof.
